buy proof in shop example skeleton & some related lemmas/tactics

ambient_capabilities_coq_model/example.v
@@ -1,6 +1,7 @@
 Require Export Arith.
 Require Import List.
 Require Import Bool.
+Require Import String.
 
 Require Import CpdtTactics.
 Require Import common.
@@ -10,6 +11,7 @@ Require Import assert.
 Require Export operational_semantics.
 Require Import assert_theory.
 Require Import hoare.
+Require Import spec.
 
 Require Export Coq.Numbers.BinNums.
 Require Export ZArith.
@@ -22,8 +24,9 @@ Module Example.
   Import SubstDefn.
   Import AssertTheory.
   Import Hoare.
+  Import SpecSatisfaction.
 
-  Declare Scope hoare_scope.
+  Open Scope hoare_scope.
   Open Scope assert_scope.
 
   (***
@@ -76,12 +79,12 @@ e : C
 
    ***)
 
-  Parameter s_minus (x y : var)(i : Z) : stmt.
+  (*)Parameter s_minus (x y : var)(i : Z) : stmt.
 
-  Parameter s_plus (x y : var)(i : Z) : stmt.
+  Parameter s_plus (x y : var)(i : Z) : stmt.*)
 
-  Parameter plus_hoare (M : module)(x y : var)(i : Z) :
-   M ⊢ {} x
+  (*Parameter plus_hoare (M : module)(x y : var)(i : Z) :=
+   M ⊢ {} x*)
 
   Definition Shop := c_id 1.
 
@@ -148,15 +151,15 @@ e : C
    *)
 
   Definition buyBody := (s_read itemPrice (e_fld (e_ item) price)) ;;
-                        ((s_read thisAcc (e_fld (e_ this) acc)) ;;
-                         ((s_read oldBalance (e_fld (e_ thisAcc) balance)) ;;
-                          ((s_call tmp buyer pay (thisAcc :: itemPrice :: nil)) ;;
-                           ((s_if (e_eq
-                                     (e_fld (e_fld (e_ this) acc) balance)
-                                     (e_plus (e_ oldBalance) (e_ itemPrice)))
-                               (s_call tmp this send (buyer :: item :: nil))
-                               (s_call tmp buyer tell nil)) ;;
-                            (s_stmt (s_ret (v_ (v_int 0)))))))).
+                        (s_read thisAcc (e_fld (e_ this) acc) ;;
+                         (s_read oldBalance (e_fld (e_ thisAcc) balance) ;;
+                          (s_call tmp buyer pay (thisAcc :: itemPrice :: nil) ;;
+                           (s_if (e_eq
+                                    (e_fld (e_fld (e_ this) acc) balance)
+                                    (e_plus (e_ oldBalance) (e_ itemPrice)))
+                              (s_call tmp this send (buyer :: item :: nil))
+                              (s_call tmp buyer tell nil) ;;
+                            ret (e_false))))).
 
   (* TODO: method specs on buy *)
   Definition buyDef := meth nil
@@ -164,9 +167,19 @@ e : C
                                (item, t_cls Item) :: nil)
                             buyBody.
 
-  Parameter sendBody : stmts.
+  Parameter sendBody : stmt.
 
-  Definition ShopMths := ⟦ buy ↦ buyDef ⟧ ∅.
+  Definition sendDef := meth nil
+                          ((buyer, t_ext) ::
+                             (item, t_cls Item) :: nil)
+                          sendBody.
+
+  Definition ShopMths := ⟦ buy ↦ buyDef ⟧ ⟦ send ↦ sendDef ⟧ ∅.
+
+  Definition ShopDef := clazz Shop
+                              ShopFlds
+                              empty
+                              ShopMths.
 
   Definition to := v_id 8.
 
@@ -176,11 +189,186 @@ e : C
 
   Definition transfer := mth_id 4.
 
-  Definition tranferBody :=
-    (s_if (e_eq (e_fld (e_ this) key) (e_ k))
-       (s_write this balance (e_minus (e_fld (e_ this) balance) (e_ amt)) ;;
-        (s_stmt (s_write to balance (e_plus (e_fld (e_ to) balance) (e_ amt)))))
-       (s_ret (v_ (v_int 0)))) ;;
-    (s_stmt (s_ret (v_ (v_int 0)))).
+  Definition transferBody :=
+    s_if (e_eq (e_fld (e_ this) key) (e_ k))
+      (s_write this balance (e_minus (e_fld (e_ this) balance) (e_ amt)))
+      (s_write to balance (e_plus (e_fld (e_ to) balance) (e_ amt))) ;;
+    ret e_false.
+
+  Definition transferDef := meth nil
+                              ((to, t_cls Account) ::
+                                 (amt, t_int) :: nil)
+                              transferBody.
+
+  Definition setKey := mth_id 5.
+
+  Definition setKeyBody :=
+    s_if (e_eq (e_fld (e_ this) key) e_null)
+      (s_write this key (e_ k) ;;
+       ret e_false)
+      (ret e_false).
+
+  Definition setKeyDef := meth nil
+                            ((k, t_cls Key) :: nil)
+                            setKeyBody.
+
+  Definition AccountMths := ⟦ transfer ↦ transferDef ⟧ ⟦ setKey ↦ setKeyDef ⟧ ∅.
+
+  Definition AccountDef := clazz Account
+                             AccountFlds
+                             empty
+                             AccountMths.
+
+  Definition KeyDef := clazz Key
+                             empty
+                             empty
+                             empty.
+
+  (* Shop Specifications *)
+
+  Definition a := v_id 11.
+
+  Definition S1 := S_inv ((a, Account)::nil) (a_prt (e_fld (e_ a) key)).
+
+  Definition Mgood : module := (S1,
+                                 ⟦ Shop ↦ ShopDef ⟧
+                                   ⟦ Account ↦ AccountDef ⟧
+                                   ⟦ Key ↦ KeyDef ⟧ ∅).
+
+  Lemma destruct_Mgood :
+    forall C CDef, ⟦ C ↦ CDef ⟧_∈ snd Mgood ->
+              (C = Shop /\ CDef = ShopDef) \/
+                (C = Account /\ CDef = AccountDef) \/
+                (C = Key /\ CDef = KeyDef).
+  Proof.
+  Admitted.
+
+  Lemma destruct_shopMths :
+    forall m mDef, ⟦ m ↦ mDef ⟧_∈ c_meths ShopDef ->
+              (m = buy /\ mDef = buyDef) \/
+                (m = send /\ mDef = sendDef).
+  Proof.
+  Admitted.
+
+  Lemma post_true :
+    forall M A s, M ⊢ ⦃ A ⦄ s ⦃ a_true ⦄.
+  Proof.
+  Admitted.
+
+  Ltac apply_hq_sequ_with_mid_eq_fst :=
+    match goal with
+      [|- _ ⊢ ⦃ ?A ⦄ _ ;; _ ⦃ _ ⦄ || ⦃ _ ⦄] => apply hq_sequ with (A2:=A)
+    end.
+
+  Ltac simpl_types :=
+    unfold a_typs;
+    unfold asrt_frm_list;
+    simpl in *.
+
+  Open Scope string_scope.
+
+  Lemma entails_refl :
+    forall M A, M ⊢ A ⊆ A.
+  Proof.
+  Admitted.
+
+  #[global] Hint Resolve entails_refl : assert_db.
+
+  Ltac hq_conj_post_conseq :=
+    match goal with
+      | [|- _ ⊢ ⦃ ?A1 ⦄ _ ⦃ ?A2 ∧ ?A3 ⦄ || ⦃ ?A ⦄ ] =>
+          apply hq_conseq with (A4:=A1)(A5:=A2)(A6:=A)
+    end.
+
+  Lemma entails_assoc1 :
+    forall M A1 A2 A3, M ⊢ ((A1 ∧ A2) ∧ A3) ⊆ (A1 ∧ (A2 ∧ A3)). Admitted.
+
+  Lemma entails_assoc2 :
+    forall M A1 A2 A3, M ⊢ (A1 ∧ (A2 ∧ A3)) ⊆ ((A1 ∧ A2) ∧ A3). Admitted.
+
+  Lemma entails_trans :
+    forall M A1 A2 A3, M ⊢ A1 ⊆ A2 ->
+                  M ⊢ A2 ⊆ A3 ->
+                  M ⊢ A1 ⊆ A3.
+  Admitted.
+
+
+  Ltac simpl_conj_entails :=
+    repeat try (eapply entails_trans; [solve [apply entails_assoc1] |]);
+    repeat try (eapply entails_trans; [|solve [apply entails_assoc2]]).
+
+  Lemma hq_conj_assoc1 :
+    forall M A1 A2 A3 A4 s A, M ⊢ ⦃ A1 ∧ (A2 ∧ A3) ⦄ s ⦃ A4 ⦄ || ⦃ A ⦄ ->
+                         M ⊢ ⦃ (A1 ∧ A2) ∧ A3 ⦄ s ⦃ A4 ⦄ || ⦃ A ⦄.
+  Proof.
+  Admitted.
+
+  Lemma hq_conj_assoc2 :
+    forall M A1 A2 A3 A4 s A, M ⊢ ⦃ A1 ⦄ s ⦃ A2 ∧ (A3 ∧ A4) ⦄ || ⦃ A ⦄ ->
+                         M ⊢ ⦃ A1 ⦄ s ⦃ (A2 ∧ A3) ∧ A4 ⦄ || ⦃ A ⦄.
+  Proof.
+  Admitted.
+
+  Ltac simpl_conj :=
+    repeat apply hq_conj_assoc1;
+    repeat apply hq_conj_assoc2.
+
+  Fixpoint contains {A : Type}`{Eq A}(l : list A)(a : A) :=
+    match l with
+    | nil => false
+    | h :: t => eqb a h || contains t a
+    end.
+
+  Fixpoint remove (A : asrt)(removed : list asrt) :=
+    match A with
+    | a_exp _ => if  then
+                  (a_true, A1 :: removed)
+    end.
+
+  Fixpoint conj_simplify A :=
+    match A with
+    | A1 \
+
+  Lemma hq_pre_dup :
+    forall M A1 A2 A3
+
+  Lemma I1 :
+    spec_sat Mgood S1.
+  Proof.
+    apply spec_invariant.
+    intros.
+    apply destruct_Mgood in H;
+      destruct H.
+
+    * (* Shop *)
+      destruct H; subst.
+      apply destruct_shopMths in H0;
+        destruct H0.
+      ** (* buy *)
+        destruct H;
+          subst.
+        simpl.
+        unfold buyBody.
+
+        apply_hq_sequ_with_mid_eq_fst.
+        *** (* itemPrice = item.price *)
+          simpl_types.
+          simpl_conj.
+          hq_conj_post_conseq;
+            eauto with assert_db.
+          
+
+        ***
+          simpl_types.
+          repeat apply hq_combine;
+            try solve [apply hq_mid, post_true].
+
+          ****
+            admit.
+
+
+
+
+  Qed.
 
 End Example.
